pulse/src/checker/Pulse.Checker.Base.fsti
@@ -262,4 +262,4 @@ val compose_checker_result_t
 : T.Tac (checker_result_t g ctxt post_hint)
 
 val infer_post #g #ctxt (r:checker_result_t g ctxt None)
-: T.Tac (post_hint_for_env g)
+: T.Tac (p:post_hint_for_env g {p.g == g /\ p.effect_annot==EffectAnnotSTT})
